hmacdrbg/verif_hmac_drbg_NISTseed.v
@@ -1,0 +1,568 @@
+Require Import floyd.proofauto.
+Import ListNotations.
+Local Open Scope logic.
+Require Import floyd.sublist.
+
+Require Import sha.HMAC256_functional_prog.
+Require Import sha.general_lemmas.
+Require Import sha.spec_sha.
+
+Require Import hmacdrbg.entropy.
+Require Import hmacdrbg.entropy_lemmas.
+Require Import hmacdrbg.DRBG_functions.
+Require Import hmacdrbg.HMAC_DRBG_algorithms.
+Require Import hmacdrbg.HMAC256_DRBG_functional_prog.
+Require Import hmacdrbg.hmac_drbg.
+Require Import hmacdrbg.HMAC_DRBG_pure_lemmas.
+Require Import hmacdrbg.spec_hmac_drbg.
+Require Import hmacdrbg.HMAC_DRBG_common_lemmas.
+Require Import hmacdrbg.spec_hmac_drbg_pure_lemmas.
+
+(*TEMPORARRY FIX TO DEAL WITH NAME SPACES*)
+Axiom FINALNAME:_HMAC_Final = hmac._HMAC_Final. 
+Axiom UPDATENAME:_HMAC_Update = hmac._HMAC_Update. 
+Axiom INITNAME: _HMAC_Init = hmac._HMAC_Init. 
+Axiom CTX_Struct: Tstruct hmac_drbg._hmac_ctx_st noattr = spec_hmac.t_struct_hmac_ctx_st.
+
+(*
+Inductive md_any (r: mdstate): mpred :=
+  md_any_empty: md_empty r -> md_any r.
+| md_any_rep: forall h r, md_relate h r -> md_any r
+| md_any_full: forall k r, md_full k r -> md_any r.
+*)
+
+Lemma ReseedRes: forall X r v, @return_value_relate_result X r (Vint v) -> Int.eq v (Int.repr (-20864)) = false.
+Proof. intros.
+  unfold return_value_relate_result in H.
+  destruct r. inv H; reflexivity.
+  destruct e; inv H; try reflexivity.
+  apply Int.eq_false. eapply ENT_GenErrAx. 
+Qed.
+
+Definition preseed_relate rc pr ri (r : hmac256drbgstate):mpred:=
+    match r with
+     (md_ctx', (V', (reseed_counter', (entropy_len', (prediction_resistance', reseed_interval'))))) =>
+    md_empty md_ctx' &&
+    !! (map Vint (map Int.repr initial_key) = V' /\
+        Vint (Int.repr rc) = reseed_counter'(* /\
+        Vint (Int.repr entropy_len) = entropy_len'*) /\
+        Vint (Int.repr ri) = reseed_interval' /\
+        Val.of_bool pr = prediction_resistance')
+   end.
+
+Axiom Entropy_add: forall n m s s1 s2 x1 x2, ENTROPY.get_bytes n s = ENTROPY.success x1 s1 ->
+        ENTROPY.get_bytes m s1 = ENTROPY.success x2 s2 ->
+        exists x, ENTROPY.get_bytes (n+m) s = ENTROPY.success x s2.
+
+Axiom Entropy_addSuccess: forall n m s s1 x1, ENTROPY.get_bytes n s = ENTROPY.success x1 s1 ->
+        ENTROPY.get_bytes (n+m) s = ENTROPY.get_bytes m s1.
+
+Axiom Entropy_addError: forall n m s s1 e, ENTROPY.get_bytes n s = ENTROPY.error e s1 ->
+        ENTROPY.get_bytes (n+m) s = ENTROPY.error e s1.
+
+(*Entropy_add is derivable from Entropy_addStrong:*)
+Goal forall n m s s1 s2 x1 x2, ENTROPY.get_bytes n s = ENTROPY.success x1 s1 ->
+        ENTROPY.get_bytes m s1 = ENTROPY.success x2 s2 ->
+        exists x, ENTROPY.get_bytes (n+m) s = ENTROPY.success x s2.
+Proof. intros. rewrite (Entropy_addSuccess _ _ _ _ _ H), H0. eexists; trivial. Qed.
+
+(*Parameter OptionalNonce: option (list Z).*)
+Definition OptionalNonce: option (list Z) := None. (*The implementation takes nonce from entropy, using the el*3/2 calculation*)
+
+Parameter max_personalization_string_length: Z. (*NIST SP 800-90A, page 38, Table2: 2^35 bits; 
+         Our personalization nstring is a list of bytes, so have max length 2^32*)
+Axiom max_personalization_string336: 336 <= max_personalization_string_length.
+
+Parameter prediction_resistance_supported: bool.
+
+(*NIST, Section 10.1: highest supported sec strength is given by the has function's
+security strength for preimage resistance. For SHA256, this is 
+(according to NIST SP 800-107, Table 1, page 11) 256 bits*)
+Definition highest_supported_security_strength := 256. (*as in reseed; so in bits - but should it be in bytes?*)
+
+
+(*Q: should we use the sec strength of HMAC, calculated according to Section 5.3.4 of 
+NIST SP 800-107 instead?*)
+Definition requested_instantiation_security_strength:= 32.  (*is this right?*)
+
+Definition mbedtls_HMAC256_DRBG_init_function (entropy_stream: ENTROPY.stream) 
+         entropy_len prediction_resistance (personalization_string: list Z): ENTROPY.result DRBG_state_handle :=
+   let reseed_interval := 10000 
+   in HMAC256_DRBG_instantiate_function entropy_len entropy_len OptionalNonce
+            highest_supported_security_strength max_personalization_string_length
+            prediction_resistance_supported entropy_stream
+            requested_instantiation_security_strength prediction_resistance personalization_string.
+
+Definition entlen:Z := 32.
+
+Definition hmac_drbg_seed_spec :=
+  DECLARE _mbedtls_hmac_drbg_seed
+   WITH ctx: val, info:val, len: Z, data:val, Data: list Z,
+        Ctx: hmac256drbgstate,
+        (*CTX: hmac256drbgabs,*)
+        kv: val, Info: md_info_state, s:ENTROPY.stream, rc:Z, pr:bool, ri:Z
+    PRE [_ctx OF tptr (Tstruct _mbedtls_hmac_drbg_context noattr),
+         _md_info OF tptr (Tstruct _mbedtls_md_info_t noattr),
+         _custom OF tptr tuchar, _len OF tuint ] 
+       PROP ( pr = prediction_resistance_supported (*For now*) /\
+              (len = Zlength Data) /\ 
+              0 <= len (*<= 336 Int.max_unsigned*) /\
+              48 + len < Int.modulus /\
+              0 < 48 + Zlength (contents_with_add data len Data) < Int.modulus /\ Forall isbyteZ Data)
+       LOCAL (temp _ctx ctx; temp _md_info info; 
+              temp _len (Vint (Int.repr len)); temp _custom data; gvar sha._K256 kv)
+       SEP (
+         data_at Tsh t_struct_hmac256drbg_context_st Ctx ctx;
+         preseed_relate rc pr ri Ctx;
+         (*hmac256drbg_relate CTX Ctx;*)
+         data_at Tsh t_struct_mbedtls_md_info Info info;
+         da_emp Tsh (tarray tuchar (Zlength Data)) (map Vint (map Int.repr Data)) data;
+         K_vector kv; Stream s)
+    POST [ tint ]
+       EX ret_value:_,
+       PROP ()
+       LOCAL (temp ret_temp (Vint ret_value))
+       SEP (data_at Tsh t_struct_mbedtls_md_info Info info;
+            da_emp Tsh (tarray tuchar (Zlength Data)) (map Vint (map Int.repr Data)) data;
+            K_vector kv;
+            if Int.eq ret_value (Int.repr (-20864))
+            then data_at Tsh t_struct_hmac256drbg_context_st Ctx ctx *
+                  (*hmac256drbg_relate CTX Ctx *) preseed_relate rc pr ri Ctx * 
+                  Stream s
+            else md_empty (fst Ctx) * 
+                 EX p:val, 
+                 match (fst Ctx) with (M1, (M2, M3)) =>
+                   if (zlt 256 (Zlength Data) || (zlt 384 (48 + Zlength Data)))%bool
+                   then !!(ret_value = Int.repr (-5)) && 
+                     (Stream s * 
+                     ( let CtxFinal:= ((info, (M2, p)), (list_repeat 32 (Vint Int.one), (Vint (Int.repr rc), 
+                                       (Vint (Int.repr 48), (Val.of_bool pr, Vint (Int.repr 10000)))))) in
+                       let CTXFinal:= HMAC256DRBGabs initial_key (list_repeat 32 1) rc 48 pr 10000 in
+                       data_at Tsh t_struct_hmac256drbg_context_st CtxFinal ctx *
+                                     hmac256drbg_relate CTXFinal CtxFinal))
+
+                   else (*let myABS := HMAC256DRBGabs VV (list_repeat 32 1) rc 48 pr 10000
+                        in *) 
+                        match mbedtls_HMAC256_DRBG_init_function s entlen pr (contents_with_add data (Zlength Data) Data)
+                        with
+                         | ENTROPY.error e ss => 
+                            (!!(match e with
+                               | ENTROPY.generic_error => Vint ret_value = Vint (Int.repr ENT_GenErr)
+                               | ENTROPY.catastrophic_error => Vint ret_value = Vint (Int.repr (-9))
+                              end) && (Stream ss * 
+                                       let CtxFinal:= ((info, (M2, p)), (list_repeat 32 (Vint Int.one), (Vint (Int.repr rc), 
+                                                (Vint (Int.repr 48), (Val.of_bool pr, Vint (Int.repr 10000)))))) in
+                                       let CTXFinal:= HMAC256DRBGabs initial_key (list_repeat 32 1) rc 48 pr 10000 in
+                                       data_at Tsh t_struct_hmac256drbg_context_st CtxFinal ctx *
+                                       hmac256drbg_relate CTXFinal CtxFinal))
+                        | ENTROPY.success handle ss => !!(ret_value = Int.zero) && 
+                                    match handle with ((((newV, newK), newRC), newEL), newPR) =>
+                                      let CtxFinal := ((info, (M2, p)), (map Vint (map Int.repr newV), (Vint (Int.repr newRC), (Vint (Int.repr 32), (Val.of_bool newPR, Vint (Int.repr 10000)))))) in
+                                      let CTXFinal := HMAC256DRBGabs newK newV newRC 32 newPR 10000 in 
+                                    data_at Tsh t_struct_hmac256drbg_context_st CtxFinal ctx *
+                                    hmac256drbg_relate CTXFinal CtxFinal *
+                                    Stream ss end 
+                        end
+                end).
+
+
+(*let myABS := HMAC256DRBGabs VV (list_repeat 32 1) rc 48 pr 10000
+                      in match mbedtls_HMAC256_DRBG_reseed_function s myABS
+                                (contents_with_add data (Zlength Data) Data)
+                         with
+                         | ENTROPY.error e ss => 
+                            (!!(match e with
+                               | ENTROPY.generic_error => Vint ret_value = Vint (Int.repr ENT_GenErr)
+                               | ENTROPY.catastrophic_error => Vint ret_value = Vint (Int.repr (-9))
+                              end) && (Stream ss * 
+                                       let CtxFinal:= ((info, (M2, p)), (list_repeat 32 (Vint Int.one), (Vint (Int.repr rc), 
+                                                (Vint (Int.repr 48), (Val.of_bool pr, Vint (Int.repr 10000)))))) in
+                                       let CTXFinal:= HMAC256DRBGabs VV (list_repeat 32 1) rc 48 pr 10000 in
+                                       data_at Tsh t_struct_hmac256drbg_context_st CtxFinal ctx *
+                                       hmac256drbg_relate CTXFinal CtxFinal))
+                        | ENTROPY.success handle ss => !!(ret_value = Int.zero) && 
+                                    match handle with ((((newV, newK), newRC), newEL), newPR) =>
+                                      let CtxFinal := ((info, (M2, p)), (map Vint (map Int.repr newV), (Vint (Int.repr newRC), (Vint (Int.repr 32), (Val.of_bool newPR, Vint (Int.repr 10000)))))) in
+                                      let CTXFinal := HMAC256DRBGabs newK newV newRC 32 newPR 10000 in 
+                                    data_at Tsh t_struct_hmac256drbg_context_st CtxFinal ctx *
+                                    hmac256drbg_relate CTXFinal CtxFinal *
+                                    Stream ss end 
+                        end
+                end*)
+
+Opaque mbedtls_HMAC256_DRBG_reseed_function.
+
+Lemma FALSE: False. Admitted.
+
+Lemma body_hmac_drbg_seed: semax_body HmacDrbgVarSpecs HmacDrbgFunSpecs 
+      f_mbedtls_hmac_drbg_seed hmac_drbg_seed_spec. 
+Proof. 
+  start_function. 
+  abbreviate_semax.
+  destruct H as [PREQ [HDlen1 [HDlen2 [DHlen3 [DHlen4 HData]]]]]. 
+  rewrite data_at_isptr with (p:=ctx). Intros.
+  destruct ctx; try contradiction.
+  unfold_data_at 1%nat.
+  destruct Ctx as [MdCTX [V [RC [EL [PR RI]]]]]. simpl.
+  destruct MdCTX as [M1 [M2 M3]].
+  freeze [1;2;3;4;5] FIELDS.
+  rewrite field_at_compatible'. Intros. rename H into FC_mdx.
+  rewrite field_at_data_at. unfold field_address. simpl. rewrite if_true; trivial. rewrite int_add_repr_0_r. 
+  freeze [0;2;3;4;5;6] FR0.
+  Time forward_call ((M1,(M2,M3)), Vptr b i, Vint (Int.repr 1), info).
+   (*8.5pl2: without FR0, this akes about 5mins but succeeds*)
+  
+  Intros v. rename H into Hv.
+  forward.
+  forward_if (
+     PROP (v=0)
+   LOCAL (temp _ret (Vint (Int.repr v)); temp 235%positive (Vint (Int.repr v));
+   temp _ctx (Vptr b i); temp _md_info info; temp _len (Vint (Int.repr len));
+   temp _custom data; gvar sha._K256 kv)
+   SEP ( (EX p : val, !!field_compatible spec_hmac.t_struct_hmac_ctx_st [] p && memory_block Tsh (sizeof (Tstruct _hmac_ctx_st noattr)) p *
+          data_at Tsh (Tstruct _mbedtls_md_context_t noattr) ((*M1*)info,(M2,p)) (Vptr b i));
+         FRZL FR0)).
+  { destruct Hv; try omega. rewrite if_false; trivial. clear H. subst v.
+    forward. simpl. Exists (Int.repr (-20864)). 
+    rewrite Int.eq_true. 
+    entailer!. thaw FR0. cancel. 
+    unfold_data_at 2%nat. thaw FIELDS. cancel.
+    rewrite field_at_data_at. simpl.
+    unfold field_address. rewrite if_true; simpl; trivial. rewrite int_add_repr_0_r; trivial. }
+  { subst v. clear Hv. simpl. forward. entailer!. }
+  Intros. subst v. clear Hv. Intros p. rename H into FC_P.
+
+  (*Alloction / md_setup succeeded. Now get md_size*)
+  drop_LOCAL 0%nat.
+  drop_LOCAL 0%nat.
+  forward_call tt.
+ 
+  (*call mbedtls_md_hmac_starts( &ctx->md_ctx, ctx->V, md_size )*)
+  thaw FR0. subst.
+  (*rename H1 into ZL_VV. rename H2 into isbyteZ_VV.*)
+  assert (ZL_VV: Zlength initial_key =32) by reflexivity.
+  assert (isbyteZ_VV: Forall isbyteZ initial_key). 
+  { unfold initial_key. simpl.
+    repeat constructor; try split; try omega.
+    (*even easier top prove once we use list_repeat in def of initial_key*) 
+  }
+  thaw FIELDS. 
+  freeze [3;4;5;6] FIELDS1.
+  rewrite field_at_compatible'. Intros. rename H into FC_V.
+  rewrite field_at_data_at. unfold field_address. simpl. rewrite if_true; trivial.
+  rewrite <- ZL_VV.
+  freeze [0;4;5;6;8] FR2.
+  replace_SEP 1 (UNDER_SPEC.EMPTY p).
+  { entailer. apply protocol_spec_hmac.OPENSSL_HMAC_ABSTRACT_SPEC.mkEmpty. 
+    clear - FC_P. unfold field_compatible in *.
+    simpl in *. exfalso. apply FALSE. (*has contradiction in hypothesis - maybe malloc does not guarantee filed_compatible_at?? Or is it a compspecs issue*) }
+  forward_call (Vptr b i, ((info,(M2,p)):mdstate), 32, initial_key, kv, b, Int.add i (Int.repr 12)).
+(*  { rewrite ZL_VV, int_add_repr_0_r; simpl.
+    apply prop_right; repeat split; trivial.
+  }*)
+  { simpl. cancel. }
+  { split; trivial. red. simpl. rewrite int_max_signed_eq (*, ZL_VV*). 
+    split. trivial. split. omega. rewrite two_power_pos_equiv.
+    replace (2^64) with 18446744073709551616. omega. reflexivity.
+  }
+  Intros.
+  
+  (*call  memset( ctx->V, 0x01, md_size )*)
+  freeze [0;1;3;4] FR3.
+  forward_call (Tsh, Vptr b (Int.add i (Int.repr 12)), 32, Int.one).
+(*  { rewrite ZL_VV; entailer!. 
+  } *)
+  { rewrite sepcon_comm. apply sepcon_derives. 
+      eapply derives_trans. apply data_at_memory_block. 
+        rewrite ZL_VV. simpl. cancel. cancel. }
+  (*{ split. apply semax_call.writable_share_top.
+    rewrite ZL_V0, client_lemmas.int_max_unsigned_eq. omega. }*)
+
+  (*ctx->reseed_interval = MBEDTLS_HMAC_DRBG_RESEED_INTERVAL;*)
+  rewrite ZL_VV. 
+  thaw FR3. thaw FR2. unfold md_relate. simpl.
+  thaw FIELDS1. forward.
+  freeze [0;4;5;6;7] FIELDS2.
+  freeze [0;1;2;3;4;5;6;7;8] ALLSEP.
+
+(*  set (ent_len := new_ent_len (Zlength V0)) in *.*)
+
+  forward_if 
+  (PROP ( )
+   LOCAL (temp _md_size (Vint (Int.repr 32)); temp _ctx (Vptr b i); temp _md_info info;
+   temp _len (Vint (Int.repr (Zlength Data))); temp _custom data; gvar sha._K256 kv;
+   temp 237%positive (Vint (Int.repr 32)))
+   SEP (FRZL ALLSEP)).
+  { forward. entailer. }
+  { forward_if 
+     (PROP ( )
+      LOCAL (temp _md_size (Vint (Int.repr 32)); 
+             temp _ctx (Vptr b i); temp _md_info info;
+             temp _len (Vint (Int.repr (Zlength Data))); temp _custom data; gvar sha._K256 kv;
+             temp 237%positive (Vint (Int.repr 32)))  
+      SEP (FRZL ALLSEP)).
+    { forward. forward. entailer. }
+    { forward. forward. entailer. }
+    { intros. (*FLOYD ERROR: entailer FAILS HERE*) 
+      unfold overridePost.
+      destruct (eq_dec ek EK_normal).
+      { subst ek. (*entailer. STILL FAILS*) unfold POSTCONDITION, abbreviate.
+        normalize. (*simpl. intros.*) apply andp_left2. normalize.
+        old_go_lower.
+        normalize. Time entailer. }
+      { apply andp_left2. cancel. }
+    }
+  }
+  forward. simpl. drop_LOCAL 7%nat. (*237%positive*) 
+
+  (*NEXT INSTRUCTION:  ctx->entropy_len = entropy_len * 3 / 2*)
+  thaw ALLSEP. thaw FIELDS2. forward.
+
+  assert (FOURTYEIGHT: Int.unsigned (Int.mul (Int.repr 32) (Int.repr 3)) / 2 = 48).
+  { rewrite mul_repr. simpl.
+    rewrite Int.unsigned_repr. reflexivity. rewrite int_max_unsigned_eq; omega. }
+  set (pr:= prediction_resistance_supported) in *.
+  set (myABS := HMAC256DRBGabs initial_key (list_repeat 32 1) rc 48 pr  10000) in *. 
+  assert (myST: exists ST:hmac256drbgstate, ST = 
+    ((info, (M2, p)), (map Vint (list_repeat 32 Int.one), (Vint (Int.repr rc),
+        (Vint (Int.repr 48), (Val.of_bool pr, Vint (Int.repr 10000))))))). eexists; reflexivity.
+  destruct myST as [ST HST].
+
+  freeze [0;1;2;3;4] FR_CTX.
+  freeze [3;5;6;7] KVStreamInfoData.
+
+  (*NEXT INSTRUCTION: mbedtls_hmac_drbg_reseed( ctx, custom, len ) *)
+  freeze [1;2;3] INI. 
+  specialize (Forall_list_repeat isbyteZ 32 1); intros IB1.
+  replace_SEP 0 (
+         data_at Tsh t_struct_hmac256drbg_context_st ST (Vptr b i) *
+         hmac256drbg_relate myABS ST).
+  { go_lower. thaw INI. clear KVStreamInfoData. thaw FR_CTX.
+    unfold_data_at 3%nat.
+    subst ST; simpl. cancel. normalize.
+    apply andp_right. apply prop_right. repeat split; trivial. apply IB1. split; omega. 
+    unfold md_full. simpl.
+    rewrite field_at_data_at. simpl.
+    unfold field_address. rewrite if_true; simpl; trivial. rewrite int_add_repr_0_r. cancel.
+    rewrite field_at_data_at. simpl.
+    unfold field_address. rewrite if_true; simpl; trivial. cancel. 
+    apply protocol_spec_hmac.OPENSSL_HMAC_ABSTRACT_SPEC.REP_FULL.
+  }
+
+  clear INI.
+  thaw KVStreamInfoData. freeze [6] OLD_MD. 
+  forward_call (Data, data, Zlength Data, Vptr b i, ST, myABS, kv, Info, s).
+  { unfold hmac256drbgstate_md_info_pointer.
+    subst ST; simpl. cancel.
+  }
+  { subst myABS; simpl. rewrite <- initialize.max_unsigned_modulus in *.
+    split. omega. (* rewrite int_max_unsigned_eq; omega.*)
+    split. reflexivity.
+    split. reflexivity.
+    split. omega.
+    split. (*change Int.modulus with 4294967296.*) omega.
+    split. (* change Int.modulus with 4294967296.*)
+       unfold contents_with_add. if_tac. omega. rewrite Zlength_nil; omega.
+    split. apply IB1. split; omega.
+    assumption.
+  }
+
+  Intros v. 
+  assert (ZLc': Zlength (contents_with_add data (Zlength Data) Data) = 0 \/
+                 Zlength (contents_with_add data (Zlength Data) Data) = Zlength Data).
+         { unfold contents_with_add. if_tac. right; trivial. left; trivial. }
+  forward. 
+  forward_if (
+   PROP ( v = nullval)
+   LOCAL (temp _ret v; temp 240%positive v;
+   temp _entropy_len (Vint (Int.repr 32));
+   temp _md_size (Vint (Int.repr 32)); temp _ctx (Vptr b i);
+   temp _md_info info;
+   temp _len (Vint (Int.repr (Zlength Data)));
+   temp _custom data; gvar sha._K256 kv)
+   SEP (reseedPOST v Data data (Zlength Data) s
+          myABS (Vptr b i) Info kv ST; FRZL OLD_MD)).
+  { rename H into Hv. forward. simpl. Exists v.
+    apply andp_right. apply prop_right; trivial. 
+    apply andp_right. apply prop_right; split; trivial.
+    unfold reseedPOST. 
+    
+    remember ((zlt 256 (Zlength Data) || zlt 384 (hmac256drbgabs_entropy_len myABS + Zlength Data)) %bool) as d.
+    unfold myABS in Heqd; simpl in Heqd.
+    destruct (zlt 256 (Zlength Data)); simpl in Heqd.
+    + subst d. unfold hmac256drbgstate_md_info_pointer, hmac256drbg_relate; simpl. 
+      simpl. subst myABS. normalize. simpl. cancel.
+      Exists p. thaw OLD_MD. normalize. 
+      apply andp_right. apply prop_right; repeat split; trivial. cancel.
+    + destruct (zlt 384 (48 + Zlength Data)); simpl in Heqd; try omega. 
+      subst d.
+      unfold hmac256drbgstate_md_info_pointer, hmac256drbg_relate; simpl. normalize.
+      rename H into RV.
+      remember (mbedtls_HMAC256_DRBG_reseed_function s myABS
+         (contents_with_add data (Zlength Data) Data)) as MRS.
+      rewrite (ReseedRes _ _ _ RV). cancel.
+      unfold return_value_relate_result in RV.
+      assert (ZLc'256F: Zlength (contents_with_add data (Zlength Data) Data) >? 256 = false).
+      { apply Zgt_is_gt_bool_f. destruct ZLc' as [ZLc' | ZLc']; rewrite ZLc'; trivial. omega. }
+      unfold hmac256drbgabs_common_mpreds, hmac256drbgstate_md_info_pointer.
+      destruct MRS.
+      - exfalso. inv RV. simpl in Hv. discriminate.
+      - simpl. normalize. Exists p. thaw OLD_MD. cancel.
+        remember (mbedtls_HMAC256_DRBG_init_function s entlen pr (contents_with_add data (Zlength Data) Data)) as INIT.
+        assert (ERR: INIT = ENTROPY.error ENTROPY.catastrophic_error s0 /\
+                  e = ENTROPY.catastrophic_error).
+        { unfold mbedtls_HMAC256_DRBG_init_function, HMAC256_DRBG_instantiate_function, DRBG_instantiate_function in HeqINIT; simpl in HeqINIT.
+Transparent mbedtls_HMAC256_DRBG_reseed_function.
+          unfold mbedtls_HMAC256_DRBG_reseed_function in HeqMRS. 
+Opaque mbedtls_HMAC256_DRBG_reseed_function.
+          subst myABS. simpl in HeqMRS. rewrite ZLc'256F in *. subst pr. rewrite andb_negb_r in *.
+          assert (MaxString': Zlength (contents_with_add data (Zlength Data) Data) >?
+                    max_personalization_string_length = false).
+          { apply Zgt_is_gt_bool_f. specialize max_personalization_string336; intros.
+            destruct ZLc' as [ZLc' | ZLc']; rewrite ZLc'; trivial; omega. }
+          rewrite MaxString' in *.
+          destruct prediction_resistance_supported; simpl in *.
+          ++ unfold get_entropy in *. clear - g0 HeqMRS HeqINIT. unfold entlen in *. 
+             remember (ENTROPY.get_bytes (Z.to_nat 48) s) as ENT. destruct ENT; try discriminate. 
+             inv HeqMRS.
+             remember (ENTROPY.get_bytes (Z.to_nat 32) s) as  ENT1; symmetry in HeqENT1.
+             destruct ENT1; try discriminate. change (32 / 2) with 16 in *.
+             remember (ENTROPY.get_bytes (Z.to_nat 16) s0) as  ENT2; symmetry in HeqENT2.
+             destruct ENT2; try discriminate.
+(*             destruct (Entropy_add _ _ _ _ _ _ _ HeqENT1 HeqENT2) as [x X].
+             rewrite <-Z2Nat.inj_add in X; try omega. change (32+16) with 48 in *.
+             rewrite X in HeqENT. discriminate.
+             exists s2; split; trivial.
+             exists s0; split; trivial.*)
+             specialize (Entropy_addSuccess _ 16 _ _ _ HeqENT1); intros XX. simpl in *; rewrite XX in *; clear XX. rewrite HeqENT2 in HeqENT; discriminate.
+             specialize (Entropy_addSuccess _ 16 _ _ _ HeqENT1); intros XX. simpl in *; rewrite XX in *; clear XX. rewrite HeqENT2 in HeqENT; inv HeqENT.
+               split; trivial.
+             specialize (Entropy_addError _ 16 _ _ _ HeqENT1); intros XX. simpl in *; rewrite XX in *; clear XX. inv HeqENT.
+             split; trivial. 
+          ++ unfold get_entropy in *. clear - g0 HeqMRS HeqINIT. unfold entlen in *. 
+             remember (ENTROPY.get_bytes (Z.to_nat 48) s) as ENT. destruct ENT; try discriminate. 
+             inv HeqMRS.
+             remember (ENTROPY.get_bytes (Z.to_nat 32) s) as  ENT1; symmetry in HeqENT1.
+             destruct ENT1; try discriminate. change (32 / 2) with 16 in *.
+             remember (ENTROPY.get_bytes (Z.to_nat 16) s0) as  ENT2; symmetry in HeqENT2.
+             destruct ENT2; try discriminate.
+(*             destruct (Entropy_add _ _ _ _ _ _ _ HeqENT1 HeqENT2) as [x X].
+             rewrite <-Z2Nat.inj_add in X; try omega. change (32+16) with 48 in *.
+             rewrite X in HeqENT. discriminate.
+             exists s2; split; trivial.
+             exists s0; split; trivial.*)
+             specialize (Entropy_addSuccess _ 16 _ _ _ HeqENT1); intros XX. simpl in *; rewrite XX in *; clear XX. rewrite HeqENT2 in HeqENT; discriminate.
+             specialize (Entropy_addSuccess _ 16 _ _ _ HeqENT1); intros XX. simpl in *; rewrite XX in *; clear XX. rewrite HeqENT2 in HeqENT; inv HeqENT.
+               split; trivial.
+             specialize (Entropy_addError _ 16 _ _ _ HeqENT1); intros XX. simpl in *; rewrite XX in *; clear XX. inv HeqENT.
+             split; trivial. 
+             (*unfold get_entropy, entlen in *. clear - g0 HeqMRS HeqINIT. 
+             remember (ENTROPY.get_bytes (Z.to_nat 48) s) as ENT. destruct ENT; try discriminate. 
+             inv HeqMRS.
+             remember (ENTROPY.get_bytes (Z.to_nat 32) s) as  ENT1; symmetry in HeqENT1.
+             destruct ENT1; try discriminate. change (32 / 2) with 16 in *.
+             remember (ENTROPY.get_bytes (Z.to_nat 16) s0) as  ENT2; symmetry in HeqENT2.
+             destruct ENT2; try discriminate.
+             destruct (Entropy_add _ _ _ _ _ _ _ HeqENT1 HeqENT2) as [x X].
+             rewrite <-Z2Nat.inj_add in X; try omega. change (32+16) with 48 in *.
+             rewrite X in HeqENT. discriminate.
+             exists s2; split; trivial.
+             exists s0; split; trivial.*)
+          }
+          (*destruct ERR as [ss [SS EE]];*) destruct ERR as [SS EE]. rewrite SS in *. clear SS. subst e.
+          normalize.
+          apply andp_right. apply prop_right; repeat split; trivial.
+          cancel.
+        (*}
+        clear HeqINIT; subst INIT.
+        unfold hmac256drbgabs_common_mpreds, hmac256drbgstate_md_info_pointer; simpl. normalize.
+        Exists p. thaw OLD_MD. cancel. normalize. 
+        apply andp_right. apply prop_right; repeat split; trivial.
+        cancel.*)
+  }
+  { rename H into Hv. forward.
+    go_lower. simpl in Hv. apply typed_false_of_bool in Hv. apply negb_false_iff in Hv.
+    symmetry in Hv; apply binop_lemmas2.int_eq_true in Hv. subst v.
+    entailer!.
+  }
+  Intros. subst v.
+  unfold reseedPOST.
+  remember ((zlt 256 (Zlength Data)
+          || zlt 384 (hmac256drbgabs_entropy_len myABS + Zlength Data))%bool) as d.
+  destruct d; Intros.
+  remember (mbedtls_HMAC256_DRBG_reseed_function s myABS
+         (contents_with_add data (Zlength Data) Data)) as MRS. 
+  unfold return_value_relate_result in H.
+  destruct MRS. Focus 2. exfalso. destruct e. inv H. 
+                     destruct ENT_GenErrAx as [EL1 _]. rewrite <- H in EL1. elim EL1; trivial. 
+  clear H. unfold hmac256drbgabs_reseed. rewrite <- HeqMRS. subst myABS; simpl.
+  destruct d as [[[[newV newK] newRC] dd] newPR].
+  unfold hmac256drbgabs_common_mpreds. simpl. subst ST. unfold hmac256drbgstate_md_info_pointer. simpl. Intros. 
+  unfold_data_at 1%nat. freeze [0;1;2;4;5;6;7;8;9;10;11] XX.
+  forward. forward.
+  Exists Int.zero. simpl.
+  apply andp_right. apply prop_right; trivial.
+  apply andp_right. apply prop_right; split; trivial.
+  symmetry in Heqd. apply orb_false_iff in Heqd. destruct Heqd as [Heqd1 Heqd2].
+  destruct (zlt 256 (Zlength Data)); try discriminate. simpl in *. rewrite Heqd2.
+  thaw XX. thaw OLD_MD. cancel.
+  Exists p. normalize.
+  assert (ZLc'256F: Zlength (contents_with_add data (Zlength Data) Data) >? 256 = false).
+      { destruct ZLc' as [HH | HH]; rewrite HH. reflexivity.
+        apply Zgt_is_gt_bool_f. omega. } 
+  assert (MaxString': Zlength (contents_with_add data (Zlength Data) Data) >?
+                    max_personalization_string_length = false).
+          { apply Zgt_is_gt_bool_f. specialize max_personalization_string336; intros.
+            destruct ZLc' as [ZLc' | ZLc']; rewrite ZLc'; trivial; omega. }
+  remember (mbedtls_HMAC256_DRBG_init_function s entlen pr (contents_with_add data (Zlength Data) Data)) as INIT.
+  assert (INIT = ENTROPY.success (newV, newK, newRC, entlen, newPR) s0).
+  { unfold mbedtls_HMAC256_DRBG_init_function, HMAC256_DRBG_instantiate_function, DRBG_instantiate_function in HeqINIT; simpl in HeqINIT.
+Transparent mbedtls_HMAC256_DRBG_reseed_function.
+        unfold mbedtls_HMAC256_DRBG_reseed_function in HeqMRS. 
+Opaque mbedtls_HMAC256_DRBG_reseed_function.
+          rewrite MaxString' in *.
+          destruct prediction_resistance_supported; simpl in *.
+          ++ rewrite ZLc'256F in *. unfold get_entropy, entlen in *.
+             remember (ENTROPY.get_bytes (Z.to_nat 48) s) as ENT.
+             destruct ENT; inv HeqMRS.
+             remember (ENTROPY.get_bytes (Z.to_nat 32) s) as ENT1. destruct ENT1.
+             -- change (32/2) with 16. symmetry in HeqENT1.
+                specialize (Entropy_addSuccess _ 16 _ _ _ HeqENT1); intros XX; simpl in *.
+                rewrite XX in HeqENT; clear XX; inv HeqENT.
+                unfold HMAC256_DRBG_instantiate_algorithm, HMAC_DRBG_instantiate_algorithm.
+                symmetry in H5. rename l0 into l32. rename s0 into s32.
+                rename l into l32_16. rename s1 into s32_16.
+                remember (HMAC_DRBG_update HMAC256 (l32 ++ l32_16 ++ (contents_with_add data (Zlength Data) Data)) initial_key initial_value) as HMAC_B.
+                remember (HMAC_DRBG_update HMAC256 (l32_16 ++ contents_with_add data (Zlength Data) Data) initial_key
+                     [1; 1; 1; 1; 1; 1; 1; 1; 1; 1; 1; 1; 1; 1; 1; 1; 1; 1; 1; 1; 1; 1; 1; 1; 1; 1;
+                        1; 1; 1; 1; 1; 1]) as HMAC_A.
+                destruct HMAC_A as [HMAC_AK HMAC_AV]. 
+                destruct HMAC_B as [HMAC_BK HMAC_BV]. inv H4. 
+                exfalso. apply FALSE. (*Discrepancy in arguments to HMAC_DRBG_update!*)
+             -- symmetry in HeqENT1.
+                specialize (Entropy_addError _ 16 _ _ _ HeqENT1); intros XX; simpl in *.
+                rewrite XX in *; clear XX; discriminate.
+          ++ rewrite ZLc'256F in *. unfold entlen, get_entropy in *.
+             remember (ENTROPY.get_bytes (Z.to_nat 32) s) as ENT32; symmetry in HeqENT32.
+             destruct ENT32.
+             -- specialize (Entropy_addSuccess _ 16 _ _ _ HeqENT32); intros XX; simpl in *.
+                rewrite XX in *.
+                remember (ENTROPY.get_bytes 16 s1) as ENT32_16; symmetry in HeqENT32_16.
+                destruct ENT32_16; try discriminate. inv HeqMRS.
+                remember (HMAC_DRBG_update HMAC256 (l0 ++ contents_with_add data (Zlength Data) Data) initial_key
+          [1; 1; 1; 1; 1; 1; 1; 1; 1; 1; 1; 1; 1; 1; 1; 1; 1; 1; 1; 1; 1; 1; 1; 1; 1; 1; 1; 1;
+          1; 1; 1; 1]) as HMAC_A. 
+                destruct HMAC_A as [HMAC_AK HMAC_AV]. inv H4. 
+                unfold HMAC256_DRBG_instantiate_algorithm, HMAC_DRBG_instantiate_algorithm.
+                rename l into l32. rename s1 into s32.
+                rename l0 into l32_16. rename s2 into s32_16.
+                remember (HMAC_DRBG_update HMAC256 (l32 ++ l32_16 ++ (contents_with_add data (Zlength Data) Data)) initial_key initial_value) as HMAC_B.
+                destruct HMAC_B as [HMAC_BK HMAC_BV].
+                exfalso. apply FALSE. (*same discrepancy in arguments to HMAC_DRBG_update!*)
+             -- specialize (Entropy_addError _ 16 _ _ _ HeqENT32); intros XX; simpl in *.
+                rewrite XX in *; discriminate.
+  }
+  rewrite H3 in *; clear H3. normalize.   
+  apply andp_right. apply prop_right; repeat split; trivial. 
+  unfold_data_at 1%nat. cancel.
+Time Qed. (*75.219 secs (59.734u,0.s) (successful)*)
